getting rid of protected keywords

BlockCacheSystem/BlockSystem.i.dfy
@@ -142,7 +142,8 @@ module BlockSystem {
     && forall ref | ref in succGraph :: (iset r | r in succGraph[ref]) == M.G.Successors(graph[ref])
   }
 
-  protected predicate WFSuccs(s: Variables, loc: Location)
+  /* protected */
+  predicate WFSuccs(s: Variables, loc: Location)
   {
     && WFDiskGraphOfLoc(s, loc)
     && SuccessorsAgree(
@@ -159,14 +160,16 @@ module BlockSystem {
     DiskGraph(s.disk.indirectionTables[loc], s.disk.nodes)
   }
 
-  protected function DiskGraphMap(
+  /* protected */
+  function DiskGraphMap(
       s: Variables) : imap<Location, imap<Reference, Node>>
   {
     imap loc | WFSuccs(s, loc)
         :: DiskGraphOfLoc(s, loc)
   }
 
-  protected function PersistentLoc(s: Variables) : Option<Location>
+  /* protected */
+  function PersistentLoc(s: Variables) : Option<Location>
   {
     if s.machine.Ready? then 
       Some(s.machine.persistentIndirectionTableLoc)
@@ -176,7 +179,8 @@ module BlockSystem {
       None
   }
 
-  protected function FrozenLoc(s: Variables) : Option<Location>
+  /* protected */
+  function FrozenLoc(s: Variables) : Option<Location>
   {
     if s.machine.Ready? && s.machine.frozenIndirectionTableLoc.Some?
         && s.machine.outstandingIndirectionTableWrite.None? then (
@@ -207,25 +211,29 @@ module BlockSystem {
     )
   }
 
-  protected predicate WFFrozenGraph(s: Variables)
+  /* protected */
+  predicate WFFrozenGraph(s: Variables)
   {
     && s.machine.Ready?
     && s.machine.frozenIndirectionTable.Some?
     && WFDiskCacheGraph(s.machine.frozenIndirectionTable.value, s.disk, s.machine.cache)
   }
 
-  protected function FrozenGraph(s: Variables) : imap<Reference, Node>
+  /* protected */
+  function FrozenGraph(s: Variables) : imap<Reference, Node>
   requires WFFrozenGraph(s)
   {
     DiskCacheGraph(s.machine.frozenIndirectionTable.value, s.disk, s.machine.cache)
   }
 
-  protected predicate UseFrozenGraph(s: Variables)
+  /* protected */
+  predicate UseFrozenGraph(s: Variables)
   {
     s.machine.Ready? && s.machine.frozenIndirectionTable.Some?
   }
 
-  protected function FrozenGraphOpt(s: Variables) : Option<imap<Reference, Node>>
+  /* protected */
+  function FrozenGraphOpt(s: Variables) : Option<imap<Reference, Node>>
   {
     if WFFrozenGraph(s) then
       Some(FrozenGraph(s))
@@ -233,31 +241,36 @@ module BlockSystem {
       None
   }
 
-  protected predicate WFLoadingGraph(s: Variables)
+  /* protected */
+  predicate WFLoadingGraph(s: Variables)
   {
     && s.machine.LoadingIndirectionTable?
     && WFDiskGraphOfLoc(s, s.machine.indirectionTableLoc)
   }
 
-  protected function LoadingGraph(s: Variables) : imap<Reference, Node>
+  /* protected */
+  function LoadingGraph(s: Variables) : imap<Reference, Node>
   requires WFLoadingGraph(s)
   {
     DiskGraphOfLoc(s, s.machine.indirectionTableLoc)
   }
 
-  protected predicate WFEphemeralGraph(s: Variables)
+  /* protected */
+  predicate WFEphemeralGraph(s: Variables)
   {
     && s.machine.Ready?
     && WFDiskCacheGraph(s.machine.ephemeralIndirectionTable, s.disk, s.machine.cache)
   }
 
-  protected function EphemeralGraph(s: Variables) : imap<Reference, Node>
+  /* protected */
+  function EphemeralGraph(s: Variables) : imap<Reference, Node>
   requires WFEphemeralGraph(s)
   {
     DiskCacheGraph(s.machine.ephemeralIndirectionTable, s.disk, s.machine.cache)
   }
 
-  protected function EphemeralGraphOpt(s: Variables) : Option<imap<Reference, Node>>
+  /* protected */
+  function EphemeralGraphOpt(s: Variables) : Option<imap<Reference, Node>>
   {
     if WFEphemeralGraph(s) then
       Some(EphemeralGraph(s))
@@ -481,7 +494,8 @@ module BlockSystem {
         reqReads[id1] != reqWrites[id2]
   }
 
-  protected predicate Inv(s: Variables)
+  /* protected */
+  predicate Inv(s: Variables)
   ensures Inv(s) ==>
     && (s.machine.Ready? ==> EphemeralGraphOpt(s).Some?)
     && M.Inv(s.machine)
